model/RearmBarrier.lean
@@ -3,6 +3,8 @@ import RearmBarrier.Basics
 import RearmBarrier.TreeModel
 import RearmBarrier.TreeProofs
 import RearmBarrier.TreeInvariant
+import RearmBarrier.TreeInit
+import RearmBarrier.StepInvariant
 import RearmBarrier.Model
 import RearmBarrier.Spec
 import RearmBarrier.Explore
